ReducibilityRecGenRules.v
@@ -24,6 +24,7 @@ Require Import Termination.EqualWithRelation.
 Require Import Termination.TermProperties.
 Require Import Termination.ErasedTermLemmas.
 Require Import Termination.OpenTOpen.
+Require Import Termination.StarInversions.
 
 Require Import Termination.Equivalence.
 Require Import Termination.EquivalenceLemmas.
@@ -35,6 +36,7 @@ Require Import Termination.ReducibilityRenaming.
 Require Import Termination.ReducibilityUnused.
 Require Import Termination.ReducibilitySubst.
 Require Import Termination.ReducibilityRecRules.
+Require Import Termination.ReducibilityNatRules.
 Require Import Termination.RedTactics.
 
 Require Import Termination.Freshness.
@@ -44,6 +46,7 @@ Require Import Termination.FVLemmasLists.
 Require Import Termination.WFLemmasLists.
 
 Require Import Termination.StrictPositivity.
+Require Import Termination.StrictPositivityLemmas.
 Require Import Termination.StrictPositivityLemma.
 Require Import Termination.StrictPositivityPush.
 Require Import Termination.StrictPositivityPull.
@@ -51,6 +54,7 @@ Require Import Termination.StrictPositivityPull.
 Require Import Omega.
 
 Opaque reducible_values.
+Opaque strictly_positive.
 Opaque makeFresh.
 
 Fixpoint build_nat (n: nat): tree :=
@@ -58,8 +62,6 @@ Fixpoint build_nat (n: nat): tree :=
   | 0 => zero
   | S n => succ (build_nat n)
   end.
-
-Definition intersect T0 Ts := T_forall T_nat (T_rec (lvar 0 term_var) T0 Ts).
 
 (*
 Definition generalizes T :=
@@ -88,17 +90,21 @@ Qed.
 
 Set Program Mode.
 
+Definition intersect T0 Ts := T_forall T_nat (T_rec (lvar 0 term_var) T0 Ts).
+
 Lemma fold_in_intersect:
-  forall theta t T,
+  forall theta t T0 Ts,
+    wf T0 0 ->
+    wf Ts 0 ->
     valid_interpretation theta ->
-    reducible_values theta t (intersect T) ->
+    reducible_values theta t (intersect T0 Ts) ->
     exists v, closed_value v /\ t = tfold v.
 Proof.
   unfold intersect;
     repeat match goal with
            | H: reducible_values _ _ (T_forall _ _) |- _ => simp reducible_values in H
-           | _ => step
-           | H: _ |- _  => apply fold_in_rec with theta T_top (open 0 T (succ zero)) zero
+           | _ => step || (rewrite open_none in * by steps)
+           | H: _ |- _  => apply fold_in_rec with theta T0 (open 0 Ts (succ zero)) zero
            | H: forall a, _ -> _ |-  _ =>
                poseNew (Mark 0 "once");
                unshelve epose proof (H (succ zero) _ _)
@@ -106,108 +112,101 @@ Proof.
            end.
 Qed.
 
+Ltac t_fold_in_intersect :=
+  match goal with
+  | H1: valid_interpretation ?theta, H2: reducible_values ?theta ?t (intersect ?T0 ?Ts) |- _ =>
+     is_var t;
+     unshelve epose proof (fold_in_intersect theta t T0 Ts _ _ H1 H2)
+  end.
+
+Lemma non_empty_nat:
+  forall theta, non_empty theta T_nat.
+Proof.
+  unfold non_empty; intros; exists zero; repeat step || simp_red.
+Qed.
+
+Ltac t_instantiate_reducible3 :=
+  match goal with
+  | H1: reducible_values _ ?v ?T, H3: forall a, _ -> _ -> _ |- _ =>
+    poseNew (Mark (v,H3) "t_instantiate_reducible");
+    unshelve epose proof (H3 v _ H1)
+  end.
+
+Lemma reducible_values_unfold_gen:
+  forall T0 Ts theta v X,
+    wf T0 0 ->
+    wf Ts 0 ->
+    twf T0 0 ->
+    twf Ts 1 ->
+    ~(X ∈ pfv Ts type_var) ->
+    strictly_positive (topen 0 Ts (fvar X type_var)) (X :: nil) ->
+    is_erased_type T0 ->
+    is_erased_type Ts ->
+    valid_interpretation theta ->
+    reducible_values theta (tfold v) (intersect T0 Ts) ->
+    reducible_values theta v (topen 0 Ts (intersect T0 Ts)).
+Proof.
+  unfold intersect in *; repeat step.
+  apply strictly_positive_push_forall2 with X;
+    repeat match goal with
+           | H: reducible_values _ _ (T_forall _ _) |- _ => simp reducible_values in H
+           | H: reducible_values _ _ (T_rec _ _ _) |- _ => simp reducible_values in H
+           | H1: reducible_values _ ?v T_nat, H3: forall a, _ -> _ -> _ |- _ =>
+             poseNew (Mark (v,H3) "t_instantiate_reducible");
+             unshelve epose proof (H3 (succ v) _ _)
+           | _ => step || (rewrite open_none in * by steps) || apply reducible_values_succ
+           end;
+      eauto using non_empty_nat;
+      eauto with berased;
+      try solve [ t_closing ];
+      eauto 3 using smallstep_succ_zero with falsity.
+
+  apply reducibility_subst_head in H19;
+    repeat step || t_invert_star || t_listutils ||
+           (rewrite is_erased_term_tfv in H15 by (eauto with berased));
+      eauto with btwf bwf.
+
+  lazymatch goal with
+  | H: star small_step ?v1 ?v2 |- _ =>
+    unshelve epose proof (star_smallstep_value v1 v2 H _); clear H2
+  end;
+    repeat step || t_listutils;
+    eauto with values.
+Qed.
+
+(*
 Ltac t_reducible_unfold :=
   match goal with
-  | _ => progress (unfold closed_value in *)
+  | _ => progress (unfold closed_value in * )
   | _ => apply star_unfold_fold
   | H: star small_step ?t (tfold ?v) |- exists t', star small_step (tunfold ?t) _ /\ _ => exists v
   | H: singleton _ = nil |- _ => inversion H
-(*  | H: reducible_values _ _ (intersect _) |- _ => simp reducible_values in H
-  | H: reducible_values _ _ (T_rec (succ zero) _ _) |- _ => simp reducible_values in H *)
+( *  | H: reducible_values _ _ (intersect _) |- _ => simp reducible_values in H
+  | H: reducible_values _ _ (T_rec (succ zero) _ _) |- _ => simp reducible_values in H * )
   | _ => step || inst_one
   | H1: valid_interpretation ?theta, H2: reducible_values ?theta ?t (intersect ?T) |- _ =>
      is_var t; pose proof (fold_in_intersect theta t T H1 H2)
   | _ => rewrite_any
   end.
+*)
 
-Lemma reducible_values_unfold_gen:
-  forall T0 Ts theta v n X,
-    wf n 0 ->
-    twf n 0 ->
+Lemma reducible_unfold_gen:
+  forall T0 Ts theta t X,
     wf T0 0 ->
-    twf T0 1 ->
     wf Ts 0 ->
+    twf T0 0 ->
     twf Ts 1 ->
-    ~(X ∈ pfv T type_var) ->
-    strictly_positive (topen 0 T (fvar X type_var)) (X :: nil) ->
-    is_erased_term n ->
-    is_erased_type T ->
+    ~(X ∈ pfv Ts type_var) ->
+    strictly_positive (topen 0 Ts (fvar X type_var)) (X :: nil) ->
+    is_erased_type T0 ->
+    is_erased_type Ts ->
     valid_interpretation theta ->
-    reducible_values theta (tfold v) (intersect T0 Ts) ->
-    reducible_values theta v (topen 0 T (intersect T0 Ts)).
+    reducible theta t (intersect T0 Ts) ->
+    reducible theta (tunfold t) (topen 0 Ts (intersect T0 Ts)).
 Proof.
-  unfold intersect in *; repeat step.
-(*  apply strictly_positive_push_forall; steps.
-  simp reducible_values in H8; steps.
-  evar (a: term).
-  unshelve epose proof (H10 (succ a) _) as HH; steps.
-  - admit.
-  - admit.
-  - simp reducible_values in HH; steps.
-    + admit.
-    + apply reducibility_subst_head in H17; steps.
-      * rewrite open_none in * by t_rewrite.
-Admitted.
-*)
-Admitted.
-
-
-(*
-  - admit.
-  - admit.
-  - simp reducible_values in H10; steps.
-    + admit.
-    + apply reducibility_subst_head in H17; steps.
-    rewrite open_topen in H17; repeat step || (rewrite open_none in * by t_rewrite); eauto with btwf. admit.
-
-  
-(*  assert (reducible_values theta v (T_forall T_nat (topen 0 T (T_rec (lvar 0 term_var) T_top T)))). { *)
-  
-    repeat match goal with
-           | H: reducible_values _ _ (T_forall _ _) |- _ => simp reducible_values in H
-           | H2: reducible_values _ ?a T_nat, H: forall a, _ -> _ |-  _ =>
-               poseNew (Mark H "instantiate once");
-               unshelve epose proof (H (succ a) _)
-           | _ =>
-             step || simp reducible_values || unfold closed_term in * ||
-             t_reducible_values_closed || unfold closed_value in * ||
-             step_inversion is_value ||
-             
-             (rewrite open_none in * by t_rewrite)
-           | H: reducible_values _ _ T_nat |- _ => simp reducible_values in H
-           | H: reducible_values ?theta (tfold ?v) (T_rec (succ ?n) ?T0 ?Ts) |- _ =>
-               poseNew (Mark H "red_once");
-               unshelve epose proof
-                 (reducible_values_unfold theta v n T0 Ts _ _ _ _ _ _ _ _ _ _ H)
-           end;
-      eauto with btwf.
-    rewrite open_topen; repeat step || (rewrite open_none in * by t_rewrite); eauto with btwf. admit.
-    lazymatch goal with
-                 | H: _ |- _ =>
-               poseNew (Mark H "red_once");
-               apply reducible_values_unfold in H
-    end.
-    apply reducible_values_unfold in H11.
-  }
-  repeat t_reducible_unfold; eauto with values.
-  repeat rewrite_any.
-  - rewrite H7 in *.
-*)
-
-Lemma reducible_unfold:
-  forall T theta t n,
-    wf n 0 ->
-    twf n 0 ->
-    wf T 0 ->
-    twf T 1 ->
-    pfv T type_var = nil ->
-    is_erased_term n ->
-    is_erased_type T ->
-    valid_interpretation theta ->
-    reducible theta t (intersect T) ->
-    reducible theta (tunfold t) (topen 0 T (intersect T)).
-Proof.
-  unfold reducible, reduces_to; repeat t_reducible_unfold; eauto with values.
-  repeat rewrite_any.
-(*  - rewrite H7 in *. *)
-Admitted.
+  unfold reducible, reduces_to;
+    repeat step || t_fold_in_intersect.
+  exists v; repeat step || apply star_unfold_fold;
+    try solve [ t_closing ];
+    eauto using reducible_values_unfold_gen.
+Qed.
